platform/tests/RosMasterDriver.v
@@ -1,0 +1,52 @@
+Require Import Ros XmlProg.
+
+Module M.
+  Definition buf_size := 1024%N.
+  Definition heapSize := (1024 * 1024 * 25)%N.
+
+  Definition ts := {| Name := "params";
+    Address := ((heapSize + 50 + 2) * 4)%N;
+    Schema := "key" :: "value" :: nil
+  |} :: nil.
+
+  Definition pr := (
+    RosCommand "setParam"(!string $"caller_id", !string $"key", !string $"value")
+    Do
+      Delete "params" Where ("key" = $"key");;
+      Insert "params" ($"key", $"value");;
+      Response Success
+        Message "Parameter set."
+        Body ignore
+      end
+    end;;
+
+    RosCommand "setParam"(!string $"caller_id", !string $"key", !int $"value")
+    Do
+      Delete "params" Where ("key" = $"key");;
+      Insert "params" ($"key", $"value");;
+      Response Success
+        Message "Parameter set."
+        Body ignore
+      end
+    end;;
+
+    RosCommand "getParamNames"(!string $"caller_id")
+    Do
+      Response Success
+        Message "Parameter names are:"
+        Body
+          ArrayFrom "params" Write
+            !string "params"#"key"
+      end
+    end
+  )%program.
+
+  Theorem Wf : wf ts pr buf_size.
+    wf.
+  Qed.
+
+  Definition port : W := 11311%N.
+  Definition numWorkers : W := 10.
+End M.
+
+Module E := Make(M).
